towards check_bbVar

src/bva/Bva_checker.v
@@ -16,9 +16,9 @@
 
 Require Import Int63 PArray.
 (*Add LoadPath "/home/burak/Desktop/smtcoq/src/bva".*)
-Require Import Misc State SMT_terms BVList.
+Require Import Misc State SMT_terms BVList Psatz.
 Require Import Bool List BoolEq NZParity.
-
+Require Import BinPos BinNat Pnat.
 Import ListNotations.
 Import Form.
 
@@ -49,7 +49,7 @@ Section Checker.
         bbT(x, [x₀; ...; xₙ₋₁])
    *)
 
-  Fixpoint check_bb (a: _lit) (bs: list _lit) (i n: nat) :=
+  Fixpoint check_bb (a: int) (bs: list _lit) (i n: nat) :=
     match bs with
     | nil => Nat_eqb i n                     (* We go up to n *)
     | b::bs =>
@@ -70,7 +70,7 @@ Section Checker.
         | _ => false
         end
       else false
-    end.
+    end.               
 
   Definition check_bbVar lres :=
     if Lit.is_pos lres then
@@ -122,7 +122,7 @@ Section Checker.
 *)
 
   (* Check the validity of a *symmetric* operator *)
-  Fixpoint check_symop (bs1 bs2 bsres : list _lit) (get_op: form -> option (_lit * _lit)) :=
+  Definition check_symop (bs1 bs2 bsres : list _lit) (get_op: form -> option (_lit * _lit)) :=
     match bs1, bs2, bsres with
     | nil, nil, nil => true
     | b1::bs1, b2::bs2, bres::bsres =>
@@ -134,7 +134,6 @@ Section Checker.
       else false
     | _, _, _ => false
     end.
-
 
 Lemma get_and_none: forall (n: int), (forall a, t_form .[ Lit.blit n] <> Fand a) ->
 (get_and (get_form (Lit.blit n))) = None.
@@ -214,7 +213,43 @@ Proof. intro a.
          case b; reflexivity.
 Qed.
 
+  Fixpoint check_symopp (bs1 bs2 bsres : list _lit) (bvop: binop) :=
+    match bs1, bs2, bsres with
+    | nil, nil, nil => true
+    | b1::bs1, b2::bs2, bres::bsres =>
+      if Lit.is_pos bres then
+        let ires := 
+        match get_form (Lit.blit bres), bvop with
+          | Fand args, BO_BVand n  =>
+            if PArray.length args == 2 then
+              let a1 := args.[0] in
+              let a2 := args.[1] in
+              ((a1 == b1) && (a2 == b2)) || ((a1 == b2) && (a2 == b1))
+            else false
 
+          | For args, BO_BVor n  =>
+            if PArray.length args == 2 then
+              let a1 := args.[0] in
+              let a2 := args.[1] in
+              ((a1 == b1) && (a2 == b2)) || ((a1 == b2) && (a2 == b1))
+            else false
+
+          | Fxor a1 a2, BO_BVxor n =>
+              ((a1 == b1) && (a2 == b2)) || ((a1 == b2) && (a2 == b1))
+                   
+          | _, _ => false
+        end in
+        if ires then check_symopp bs1 bs2 bsres bvop
+        else false
+          
+      else false
+    | _, _, _ => false
+    end.
+
+  Lemma empty_list_length: forall {A: Type} (a: list A), (length a = 0)%nat <-> a = [].
+  Proof. intros A a.
+         induction a; split; intros; auto; contradict H; easy.
+  Qed.
   (* TODO: check the first argument of BVand, BVor *)
   Definition check_bbOp pos1 pos2 lres :=
     match S.get s pos1, S.get s pos2 with
@@ -251,6 +286,44 @@ Qed.
       else C._true
     | _, _ => C._true
     end.
+
+  (* TODO: check the first argument of BVand, BVor *)
+  Definition check_bbOpp pos1 pos2 lres n :=
+    match S.get s pos1, S.get s pos2 with
+    | l1::nil, l2::nil =>
+      if (Lit.is_pos l1) && (Lit.is_pos l2) && (Lit.is_pos lres) then
+        match get_form (Lit.blit l1), get_form (Lit.blit l2), get_form (Lit.blit lres) with
+        | FbbT a1 bs1, FbbT a2 bs2, FbbT a bsres =>
+          match get_atom a with
+          | Abop (BO_BVand _) a1' a2' =>
+            if (((a1 == a1') && (a2 == a2')) || ((a1 == a2') && (a2 == a1')))
+                 && (@check_symopp bs1 bs2 bsres (BO_BVand n))
+            then lres::nil
+            else C._true
+          | Abop (BO_BVor _) a1' a2' =>
+            if (((a1 == a1') && (a2 == a2')) || ((a1 == a2') && (a2 == a1')))
+                 && (check_symopp bs1 bs2 bsres  (BO_BVor n))
+            then lres::nil
+            else C._true
+          | Abop (BO_BVxor _) a1' a2' =>
+            if (((a1 == a1') && (a2 == a2')) || ((a1 == a2') && (a2 == a1')))
+                 && (check_symopp bs1 bs2 bsres  (BO_BVxor n))
+            then lres::nil
+            else C._true
+    (*      | Abop (UO_BVneg _) a1' a2' =>
+            if (((a1 == a1') && (a2 == a2')) || ((a1 == a2') && (a2 == a1')))
+                 && (check_symop bs1 bs2 bsres get_xor)
+            then lres::nil
+            else C._true
+    *)
+       | _ => C._true
+          end
+        | _, _, _ => C._true
+        end
+      else C._true
+    | _, _ => C._true
+    end.
+
 
 Lemma bbOp0: forall pos1 pos2 lres, S.get s pos1 = [] ->  check_bbOp pos1 pos2 lres = [Lit._true].
 Proof. intros pos1 pos2 lres H0.
@@ -358,8 +431,46 @@ Qed.
     (*   apply wf_rho. *)
     (* Qed. *)
 
-    (* Let rho_interp : forall x : int, rho x = Form.interp interp_form_hatom interp_form_hatom_bv t_form (t_form.[ x]). *)
-    (* Proof. intros x;apply wf_interp_form;trivial. Qed. *)
+     Let rho_interp : forall x : int, rho x = Form.interp interp_form_hatom interp_form_hatom_bv t_form (t_form.[ x]).
+     Proof. intros x;apply wf_interp_form;trivial. Qed.
+
+(*
+Lemma prop_checkbb: forall (a: int) (bs: list _lit) (i n: nat),
+                    (check_bb a bs i n = true) ->
+                    (length bs = (n - i))%nat /\ 
+                    (forall i0, (i0 < n )%nat ->
+                    Lit.interp rho (nth i0 bs false) = 
+                    BITVECTOR_LIST.bitOf i0 (interp_form_hatom_bv a (N.of_nat n))).
+Proof.
+Admitted.
+*)
+
+Lemma prop_checkbb': forall (a: int) (bs: list _lit),
+                     (check_bb a bs 0 (length bs) = true) ->
+                     (forall i0, (i0 < (length bs) )%nat ->
+                     Lit.interp rho (nth i0 bs false) = 
+                     (@BITVECTOR_LIST.bitOf (N.of_nat(length bs)) i0 
+                     (interp_form_hatom_bv a (N.of_nat (length bs))))).
+Proof. 
+Admitted.
+
+(*
+  Lemma of_bits_bitOf: forall i l, (@BITVECTOR_LIST.bitOf (N.of_nat (length l)) i 
+                                                          (BITVECTOR_LIST.of_bits l))
+                                                           = nth i l (Lit.interp rho false).
+  Proof.
+  Admitted.
+*)
+
+Lemma bitOf_of_bits: forall l (a: BITVECTOR_LIST.bitvector (N.of_nat (length l))), 
+                               (forall i, 
+                               (i < (length l))%nat ->
+                               nth i l (Lit.interp rho false) = 
+                               (@BITVECTOR_LIST.bitOf (N.of_nat (length l)) i a))
+                               ->
+                               (BITVECTOR_LIST.bv_eq a (BITVECTOR_LIST.of_bits l)).
+Proof. 
+Admitted.
 
     Lemma valid_check_bbVar lres : C.valid rho (check_bbVar lres).
     Proof.
@@ -372,21 +483,16 @@ Qed.
       unfold Lit.interp. rewrite Heq1.
       unfold Var.interp.
       rewrite wf_interp_form; trivial. rewrite Heq0. simpl.
-      unfold BITVECTOR_LIST.bv_eq, BITVECTOR_LIST.bv.
-      simpl. destruct interp_form_hatom_bv.
-      unfold RAWBITVECTOR_LIST.bv_eq,  RAWBITVECTOR_LIST.size, RAWBITVECTOR_LIST.of_bits in *.
-      rewrite wf0. rewrite N.eqb_compare. rewrite N.compare_refl.
-      unfold RAWBITVECTOR_LIST.size, RAWBITVECTOR_LIST.bits in *.
-      unfold Valuation.wf in wf_rho.
-      unfold Lit.interp, Var.interp.
-      (* unfold BITVECTOR_LIST.bv_eq, BITVECTOR_LIST.bv. *)
-      (* simpl. destruct interp_form_hatom_bv. *)
-      (* unfold RAWBITVECTOR_LIST.bv_eq,  RAWBITVECTOR_LIST.size, RAWBITVECTOR_LIST.of_bits in *. *)
-      (* rewrite wf0. rewrite N.eqb_compare. rewrite N.compare_refl. *)
-      (* unfold RAWBITVECTOR_LIST.size, RAWBITVECTOR_LIST.bits in *. *)
-    Admitted.    
+      apply bitOf_of_bits. intros. rewrite map_nth.
+      remember (@prop_checkbb' a bs Heq2 i).
+      rewrite map_length in H.
+      rewrite map_length.
+      clear Heqe.
+      now apply e in H.
+    Qed.
 
     Lemma valid_check_bbOp pos1 pos2 lres : C.valid rho (check_bbOp pos1 pos2 lres).
+    
     Proof.
       unfold check_bbOp.
       case_eq (S.get s pos1); [intros _|intros l1 [ |l] Heq1]; try now apply C.interp_true.
@@ -402,6 +508,367 @@ Qed.
       (* BVand *)
       - case_eq ((a1 == a1') && (a2 == a2') || (a1 == a2') && (a2 == a1')); simpl; intros Heq10; try (now apply C.interp_true).
         case_eq (check_symop bs1 bs2 bsres get_and); simpl; intros Heq11; try (now apply C.interp_true).
+        unfold C.valid. simpl. rewrite orb_false_r.
+        unfold Lit.interp. rewrite Heq5.
+        unfold Var.interp.
+        rewrite wf_interp_form; trivial. rewrite Heq8. simpl.
+        unfold Atom.interp_form_hatom_bv at 2, Atom.interp_hatom.
+        rewrite Atom.t_interp_wf; trivial.
+        rewrite Heq9. simpl. unfold apply_binop.
+        case_eq (t_interp .[ a1']). intros V1 v1 Heq21.
+        case_eq (t_interp .[ a2']). intros V2 v2 Heq22.
+        admit.
+        (* rewrite Typ.neq_cast. case_eq (Typ.eqb V1 (Typ.TBV N)); simpl. *)
+        (* We need to use well-typedness information *)
+      (* BVor *)
+      - admit.
+      (* BVxor *)
+      - admit.
+    Admitted.
+
+ Lemma eq_head: forall {A: Type} a b (l: list A), (a :: l) = (b :: l) <-> a = b.
+ Proof. intros A a b l.
+        induction l as [ | l xs IHxs].
+        intros.
+        split. intros. now inversion H.
+         intros. now rewrite H.
+         intros.
+         split. intros. apply IHxs. now inversion H.
+         intros; now rewrite H.
+  Qed.
+
+Axiom afold_left_and : forall a, 
+      afold_left bool int true andb (Lit.interp rho) a = List.forallb (Lit.interp rho) (to_list a).
+
+Lemma eqb_spec : forall x y, (x == y) = true <-> x = y.
+Proof.
+ split;auto using eqb_correct, eqb_complete.
+Qed.
+
+Lemma to_list_two: forall {A:Type} (a: PArray.array A), 
+       PArray.length a = 2 -> (to_list a) = a .[0] :: a .[1] :: nil.
+Proof. intros A a H.
+       rewrite to_list_to_list_ntr. unfold to_list_ntr.
+       rewrite H.
+       cut (0 == 2 = false). intro H1.
+       rewrite H1.
+       unfold foldi_ntr. rewrite foldi_cont_lt; auto.
+       auto.
+Qed.
+
+Lemma check_symopp_and: forall ibs1 ibs2 xbs1 ybs2 ibsres zbsres n,
+      check_symopp (ibs1 :: xbs1) (ibs2 :: ybs2) (ibsres :: zbsres) (BO_BVand (N.of_nat n)) = true ->
+      check_symopp xbs1 ybs2 zbsres (BO_BVand (N.of_nat (n - 1))) = true.
+Proof. intros.
+       induction n. simpl.
+       simpl in H. 
+       case (Lit.is_pos ibsres) in H.
+       case (t_form .[ Lit.blit ibsres]) in H; try (contradict H; easy).
+       case (PArray.length a == 2) in H.
+       case ((a .[ 0] == ibs1) && (a .[ 1] == ibs2)
+         || (a .[ 0] == ibs2) && (a .[ 1] == ibs1)) in H.
+       exact H.
+       now contradict H.
+       now contradict H.
+       now contradict H.
+       simpl in H.
+       case (Lit.is_pos ibsres) in H.
+       case (t_form .[ Lit.blit ibsres]) in H; try (contradict H; easy).
+       case (PArray.length a == 2) in H.       
+       admit. (*****)
+       now contradict H.
+       now contradict H.
+Admitted.
+
+Lemma asd: forall bs1 bs2 bsres, 
+  let n := length bsres in
+  (length bs1 = n)%nat -> 
+  (length bs2 = n)%nat -> 
+  check_symopp bs1 bs2 bsres (BO_BVand (N.of_nat n)) = true ->
+  (List.map (Lit.interp rho) bsres) = 
+  (RAWBITVECTOR_LIST.map2 andb (List.map (Lit.interp rho) bs1) (List.map (Lit.interp rho) bs2)).
+Proof. intro bs1.
+         induction bs1 as [ | ibs1 xbs1 IHbs1].
+         - intros. simpl in *. rewrite <- H0 in H.
+           rewrite <- H in H0. unfold n in H0.
+           symmetry in H0.
+           rewrite empty_list_length in H0.
+           unfold map. now rewrite H0.
+         - intros [ | ibs2 ybs2].
+           + intros.
+             simpl in *. now contradict H1.
+           + intros [ | ibsres zbsres ].
+             * intros. simpl in *. now contradict H.
+             * intros. simpl.
+               specialize (IHbs1 ybs2 zbsres). 
+               rewrite IHbs1. rewrite eq_head.
+               unfold Lit.interp, Var.interp.
+               case_eq (Lit.is_pos ibsres); intro Heq0.
+               case_eq (Lit.is_pos ibs1); intro Heq1.
+               case_eq (Lit.is_pos ibs2); intro Heq2.
+               rewrite wf_interp_form; trivial.
+               simpl in H1.
+               rewrite Heq0 in H1.
+               case_eq (t_form .[ Lit.blit ibsres]).
+               try (intros i Heq; rewrite Heq in H1; now contradict H1).
+               try (intros Heq; rewrite Heq in H1; now contradict H1).
+               try (intros Heq; rewrite Heq in H1; now contradict H1).
+               try (intros i i0 Heq; rewrite Heq in H1; now contradict H1).
+               intros. rewrite H2 in H1. simpl.
+               rewrite afold_left_and.
+ 
+                case_eq (PArray.length a == 2). intros. rewrite H3 in H1.
+                rewrite eqb_spec in H3.
+                apply to_list_two in H3.
+             (*   apply length_to_list in H4. *)
+                unfold forallb.
+                rewrite H3.
+                case_eq ((a .[ 0] == ibs1) && (a .[ 1] == ibs2)). intros H5.
+                rewrite andb_true_iff in H5. destruct H5 as (H5 & H6).
+                rewrite eqb_spec in H5, H6. rewrite H5, H6.
+                unfold Lit.interp.
+                rewrite Heq1, Heq2.
+                unfold Var.interp. now rewrite andb_true_r.
+                intros. rewrite H4 in H1. simpl in *.
+                case_eq ((a .[ 0] == ibs2) && (a .[ 1] == ibs1)).
+                intros H5.
+                rewrite andb_true_iff in H5. destruct H5 as (H5 & H6).
+                rewrite eqb_spec in H5, H6.
+                rewrite H5, H6. rewrite andb_true_r.
+                unfold Lit.interp.
+                rewrite Heq1, Heq2.
+                unfold Var.interp. now rewrite andb_comm.
+                intros. rewrite H5 in H1. now contradict H1.
+                intros. rewrite H3 in H1. now contradict H1.
+              
+              try (intros a Heq; rewrite Heq in H1; now contradict H1).
+              try (intros a Heq; rewrite Heq in H1; now contradict H1).
+              try (intros i i0 Heq; rewrite Heq in H1; now contradict H1).
+              try (intros i i0 Heq; rewrite Heq in H1; now contradict H1).
+              try (intros i i0 i1 Heq; rewrite Heq in H1; now contradict H1).
+              try (intros i l Heq; rewrite Heq in H1; now contradict H1).
+
+              rewrite wf_interp_form; trivial. simpl in H1.
+              case_eq (t_form .[ Lit.blit ibsres]).
+              rewrite Heq0 in H1.
+              case_eq (t_form .[ Lit.blit ibsres]).
+               try (intros i Heq; rewrite Heq in H1; now contradict H1).
+               try (intros Heq; rewrite Heq in H1; now contradict H1).
+               try (intros Heq; rewrite Heq in H1; now contradict H1).
+               try (intros i i0 Heq; rewrite Heq in H1; now contradict H1).
+               intros. contradict H3. discriminate.
+               intros. contradict H3. discriminate.
+               intros. contradict H3. discriminate.
+               intros. contradict H3. discriminate.
+               intros. contradict H3. discriminate.
+               intros. contradict H3. discriminate.
+               intros. contradict H3. discriminate.
+               rewrite Heq0 in H1.
+               try (intros Heq; rewrite Heq in H1; now contradict H1).
+               rewrite Heq0 in H1.
+               try (intros Heq; rewrite Heq in H1; now contradict H1).
+               rewrite Heq0 in H1.
+               try (intros i i0 Heq; rewrite Heq in H1; now contradict H1).
+               rewrite Heq0 in H1.
+               try (intros a Heq; rewrite Heq in H1; now contradict H1).
+               intros. rewrite H2 in H1. simpl.
+               rewrite afold_left_and.
+
+                case_eq (PArray.length a == 2). intros. rewrite H3 in H1.
+                rewrite eqb_spec in H3.
+                apply to_list_two in H3.
+             (*   apply length_to_list in H3. *)
+                unfold forallb.
+                rewrite H3.
+                case_eq ((a .[ 0] == ibs1) && (a .[ 1] == ibs2)). intros H5.
+                rewrite andb_true_iff in H5. destruct H5 as (H5 & H6).
+                rewrite eqb_spec in H5, H6. rewrite H5, H6.
+                unfold Lit.interp.
+                rewrite Heq1, Heq2.
+                unfold Var.interp. now rewrite andb_true_r.
+                intros H4. rewrite H4 in H1. simpl in *.
+                case_eq ((a .[ 0] == ibs2) && (a .[ 1] == ibs1)). intros H5.
+                rewrite andb_true_iff in H5. destruct H5 as (H6 & H7).
+                rewrite eqb_spec in H6, H7.
+                rewrite H6, H7. rewrite andb_true_r.
+                unfold Lit.interp.
+                rewrite Heq1, Heq2.
+                unfold Var.interp. now rewrite andb_comm.
+                intros. rewrite H5 in H1. now contradict H1.
+                intros. rewrite H3 in H1. now contradict H1.
+
+               rewrite Heq0 in H1.
+               try (intros a Heq; rewrite Heq in H1; now contradict H1).
+               rewrite Heq0 in H1.
+               try (intros a Heq; rewrite Heq in H1; now contradict H1).
+               rewrite Heq0 in H1.
+               try (intros i i0 Heq; rewrite Heq in H1; now contradict H1).
+               rewrite Heq0 in H1.
+               try (intros i i0 Heq; rewrite Heq in H1; now contradict H1).
+               rewrite Heq0 in H1.
+               try (intros i i0 i1 Heq; rewrite Heq in H1; now contradict H1).
+               rewrite Heq0 in H1.
+               try (intros i l Heq; rewrite Heq in H1; now contradict H1).
+
+               case_eq (Lit.is_pos ibs2).
+               intro Heq2.
+
+              rewrite wf_interp_form; trivial. simpl in H1.
+              case_eq (t_form .[ Lit.blit ibsres]).
+              rewrite Heq0 in H1.
+              case_eq (t_form .[ Lit.blit ibsres]).
+               try (intros i Heq; rewrite Heq in H1; now contradict H1).
+               try (intros Heq; rewrite Heq in H1; now contradict H1).
+               try (intros Heq; rewrite Heq in H1; now contradict H1).
+               try (intros i i0 Heq; rewrite Heq in H1; now contradict H1).
+               intros. contradict H3. discriminate.
+               intros. contradict H3. discriminate.
+               intros. contradict H3. discriminate.
+               intros. contradict H3. discriminate.
+               intros. contradict H3. discriminate.
+               intros. contradict H3. discriminate.
+               intros. contradict H3. discriminate.
+               rewrite Heq0 in H1.
+               try (intros Heq; rewrite Heq in H1; now contradict H1).
+               rewrite Heq0 in H1.
+               try (intros Heq; rewrite Heq in H1; now contradict H1).
+               rewrite Heq0 in H1.
+               try (intros i i0 Heq; rewrite Heq in H1; now contradict H1).
+               rewrite Heq0 in H1.
+               try (intros a Heq; rewrite Heq in H1; now contradict H1).
+               intros. rewrite H2 in H1. simpl.
+               rewrite afold_left_and.
+                
+                case_eq (PArray.length a == 2). intros. rewrite H3 in H1.
+                rewrite eqb_spec in H3.
+                apply to_list_two in H3.
+             (*   apply length_to_list in H3. *)
+                unfold forallb.
+                rewrite H3.
+                case_eq ((a .[ 0] == ibs1) && (a .[ 1] == ibs2)). intros H5.
+                rewrite andb_true_iff in H5. destruct H5 as (H5 & H6).
+                rewrite eqb_spec in H5, H6. rewrite H5, H6.
+                unfold Lit.interp.
+                rewrite Heq1, Heq2.
+                unfold Var.interp. now rewrite andb_true_r.
+                intros. rewrite H4 in H1. simpl in *.
+                case_eq ((a .[ 0] == ibs2) && (a .[ 1] == ibs1)). intros H5.
+                rewrite andb_true_iff in H5. destruct H5 as (H6 & H7).
+                rewrite eqb_spec in H6, H7.
+                rewrite H6, H7. rewrite andb_true_r.
+                unfold Lit.interp.
+                rewrite Heq1, Heq2.
+                unfold Var.interp. now rewrite andb_comm.
+                intros. rewrite H5 in H1. now contradict H1.
+                intros. rewrite H3 in H1. now contradict H1.
+              
+              rewrite Heq0 in H1.
+              try (intros a Heq; rewrite Heq in H1; now contradict H1).
+              rewrite Heq0 in H1.
+              try (intros a Heq; rewrite Heq in H1; now contradict H1).
+              rewrite Heq0 in H1.
+              try (intros i i0 Heq; rewrite Heq in H1; now contradict H1).
+              rewrite Heq0 in H1.
+              try (intros i i0 Heq; rewrite Heq in H1; now contradict H1).
+              rewrite Heq0 in H1.
+              try (intros i i0 i1 Heq; rewrite Heq in H1; now contradict H1).
+              rewrite Heq0 in H1.
+              try (intros i l Heq; rewrite Heq in H1; now contradict H1).
+              
+              intros.
+
+              rewrite wf_interp_form; trivial. simpl in H1.
+              case_eq (t_form .[ Lit.blit ibsres]).
+              rewrite Heq0 in H1.
+              case_eq (t_form .[ Lit.blit ibsres]).
+               try (intros i Heq; rewrite Heq in H1; now contradict H1).
+               try (intros Heq; rewrite Heq in H1; now contradict H1).
+               try (intros Heq; rewrite Heq in H1; now contradict H1).
+               try (intros i i0 Heq; rewrite Heq in H1; now contradict H1).
+               intros. contradict H3. discriminate.
+               intros. contradict H3. discriminate.
+               intros. contradict H3. discriminate.
+               intros. contradict H3. discriminate.
+               intros. contradict H3. discriminate.
+               intros. contradict H3. discriminate.
+               intros. contradict H3. discriminate.
+               rewrite Heq0 in H1.
+               try (intros Heq; rewrite Heq in H1; now contradict H1).
+               rewrite Heq0 in H1.
+               try (intros Heq; rewrite Heq in H1; now contradict H1).
+               rewrite Heq0 in H1.
+               try (intros i i0 Heq; rewrite Heq in H1; now contradict H1).
+               rewrite Heq0 in H1.
+               try (intros a Heq; rewrite Heq in H1; now contradict H1).
+               intros. rewrite H3 in H1. simpl.
+               rewrite afold_left_and.
+
+               case_eq (PArray.length a == 2). intros H5.
+                rewrite H5 in H1.
+                rewrite eqb_spec in H5.
+                apply to_list_two in H5.
+             (*   apply length_to_list in H3. *)
+                unfold forallb.
+                rewrite H5.
+                case_eq ((a .[ 0] == ibs1) && (a .[ 1] == ibs2)). intros H6.
+                rewrite andb_true_iff in H6. destruct H6 as (H6 & H7).
+                rewrite eqb_spec in H6, H7. rewrite H6, H7.
+                unfold Lit.interp.
+                rewrite Heq1, H2.
+                unfold Var.interp. now rewrite andb_true_r.
+                intros H6. rewrite H6 in H1. simpl in *.
+                case_eq ((a .[ 0] == ibs2) && (a .[ 1] == ibs1)). intros H7.
+                rewrite andb_true_iff in H7. destruct H7 as (H7 & H8).
+                rewrite eqb_spec in H7, H8.
+                rewrite H7, H8. rewrite andb_true_r.
+                unfold Lit.interp.
+                rewrite Heq1, H2.
+                unfold Var.interp. now rewrite andb_comm.
+                intros. rewrite H4 in H1. now contradict H1.
+                intros. rewrite H4 in H1. now contradict H1.
+            
+
+              rewrite Heq0 in H1.
+              try (intros a Heq; rewrite Heq in H1; now contradict H1).
+              rewrite Heq0 in H1.
+              try (intros a Heq; rewrite Heq in H1; now contradict H1).
+              rewrite Heq0 in H1.
+              try (intros i i0 Heq; rewrite Heq in H1; now contradict H1).
+              rewrite Heq0 in H1.
+              try (intros i i0 Heq; rewrite Heq in H1; now contradict H1).
+              rewrite Heq0 in H1.
+              try (intros i i0 i1 Heq; rewrite Heq in H1; now contradict H1).
+              rewrite Heq0 in H1.
+              try (intros i l Heq; rewrite Heq in H1; now contradict H1).
+
+              rewrite wf_interp_form; trivial. simpl in H1.
+              rewrite Heq0 in H1. now contradict H1.
+              now inversion H.
+              now inversion H0.
+              remember (@check_symopp_and ibs1 ibs2 xbs1 ybs2 ibsres zbsres).
+              cut ((length zbsres = (n - 1))%nat). intros. rewrite H2.
+              apply (@check_symopp_and ibs1 ibs2 xbs1 ybs2 ibsres zbsres).
+              exact H1.
+              unfold n. simpl. omega.
+Qed.  
+ 
+   Lemma valid_check_bbOpp pos1 pos2 lres n: C.valid rho (check_bbOpp pos1 pos2 lres n).
+    Proof.
+      unfold check_bbOpp.
+      case_eq (S.get s pos1); [intros _|intros l1 [ |l] Heq1]; try now apply C.interp_true.
+      case_eq (S.get s pos2); [intros _|intros l2 [ |l] Heq2]; try now apply C.interp_true.
+      case_eq (Lit.is_pos l1); intro Heq3; simpl; try now apply C.interp_true.
+      case_eq (Lit.is_pos l2); intro Heq4; simpl; try now apply C.interp_true.
+      case_eq (Lit.is_pos lres); intro Heq5; simpl; try now apply C.interp_true.
+      case_eq (t_form .[ Lit.blit l1]); try (intros; now apply C.interp_true). intros a1 bs1 Heq6.
+      case_eq (t_form .[ Lit.blit l2]); try (intros; now apply C.interp_true). intros a2 bs2 Heq7.
+      case_eq (t_form .[ Lit.blit lres]); try (intros; now apply C.interp_true).
+      intros a bsres Heq8.
+      case_eq (t_atom .[ a]); try (intros; now apply C.interp_true).
+      intros [ | | | | | | |A|N|N|N|N|N|N] a1' a2' Heq9; try now apply C.interp_true.
+      (* BVand *)
+      - case_eq ((a1 == a1') && (a2 == a2') || (a1 == a2') && (a2 == a1')); simpl; intros Heq10; try (now apply C.interp_true).
+        case_eq (check_symopp bs1 bs2 bsres (BO_BVand n)); simpl; intros Heq11; try (now apply C.interp_true).
         unfold C.valid. simpl. rewrite orb_false_r.
         unfold Lit.interp. rewrite Heq5.
         unfold Var.interp.
